Prove lemmas need for stack monoid

F_mu_ref_par/examples/stack/rules.v
@@ -1,11 +1,20 @@
 From iris.proofmode Require Import invariants ghost_ownership tactics.
-From F_mu_ref_par Require Import lang examples.lock typing
-     logrel_binary fundamental_binary rules_binary rules.
-From iris.algebra Require Import gmap dec_agree auth.
+From F_mu_ref_par Require Import lang rules logrel_binary.
+From iris.algebra Require Import gmap dec_agree auth upred_big_op.
 From iris.program_logic Require Import ownership auth.
 Import uPred.
 
 Definition stackR : cmraT := gmapR loc (dec_agreeR val).
+
+Lemma stackR_self_op (h : stackR) : h ≡ h ⋅ h.
+Proof.
+  intros i. rewrite lookup_op.
+  match goal with
+    |- ?A ≡ ?B ⋅ ?B => change B with A; destruct A as [c|]
+  end; trivial.
+  destruct c as [c|]; cbv -[equiv decide];
+    try destruct decide; trivial; tauto.
+Qed.
 
 Class stackG Σ :=
   StackG {
@@ -16,28 +25,162 @@ Class stackG Σ :=
 Section Rules.
   Context {Σ : gFunctors} {istk : stackG Σ}.
 
-  Lemma stackR_self_op (h : stackR) : h ≡ h ⋅ h.
+  Definition stack_mapsto (l : loc) (v: val) : iPropG lang Σ :=
+    auth_own stack_name ({[ l := (DecAgree v) ]}).
+
+  Notation "l ↦ˢᵗᵏ v" := (stack_mapsto l v) (at level 20) : uPred_scope.
+
+  Lemma stack_mapsto_dup l v : True%I ⊢ (l ↦ˢᵗᵏ v -★ (l ↦ˢᵗᵏ v ★ l ↦ˢᵗᵏ v))%I.
   Proof.
-    intros i. rewrite lookup_op.
-    match goal with
-      |- ?A ≡ ?B ⋅ ?B => change B with A; destruct A as [c|]
-    end; trivial.
-    destruct c as [c|];
-      unfold op, cmra_op; simpl;
-          unfold op, cmra_op; simpl; trivial;
-            destruct decide; trivial; tauto.
+    iIntros "H".
+    unfold stack_mapsto, auth_own.
+    rewrite -own_op -auth_frag_op.
+    rewrite -stackR_self_op; trivial.
   Qed.
 
-  Lemma stackR_get_auth (h : stackR) : (● h) ~~> (● h ⋅ ◯ h).
+  Program Definition StackLink_pre (Q : bivalC -n> iPropG lang Σ)
+    {HQ : BiVal_to_IProp_Persistent Q} :
+    (bivalC -n> iPropG lang Σ) -n> bivalC  -n> iPropG lang Σ :=
+    {|
+      cofe_mor_car :=
+        λ P,
+        {|
+          cofe_mor_car :=
+            λ v, (∃ l w, v.1 = LocV l ★ l ↦ˢᵗᵏ w ★
+                                    ((w = InjLV UnitV ∧ v.2 = InjLV UnitV) ∨
+                                     (∃ y1 z1 y2 z2,
+                                         (w = InjRV (PairV y1 z1))
+                                           ★ (v.2 = InjRV (PairV y2 z2))
+                                           ★ Q (y1, y2) ★ ▷ P(z1, z2)
+                                     )
+                                    )
+                 )%I
+        |}
+    |}.
+  Next Obligation.
   Proof.
-    intros n z H1. destruct z as [[ze | |] zo];
-    unfold validN, cmra_validN in *; simpl in *; trivial.
-    destruct H1 as [H1 H2]; split; trivial.
-    destruct H1 as [u H1].
-    eexists u. rewrite H1.
-    rewrite ?cmra_unit_left_id.
-    rewrite -assoc.
-      by rewrite -stackR_self_op.
+    intros Q HQ P n [v1 v2] [w1 w2] [Hv1 Hv2]; simpl in *;
+      by rewrite Hv1 Hv2.
+  Qed.
+  Next Obligation.
+  Proof.
+    intros Q HQ n P1 P2 HP v; simpl in *.
+    repeat (apply exist_ne => ?). repeat apply sep_ne; trivial.
+    rewrite or_ne; trivial. repeat (apply exist_ne => ?).
+      by rewrite HP.
+  Qed.
+
+  Global Instance StackLink_pre_contractive Q {HQ} :
+    Contractive (@StackLink_pre Q HQ).
+  Proof.
+    intros n P1 P2 HP v; simpl. repeat (apply exist_ne => ?).
+    repeat apply sep_ne; trivial. rewrite or_ne; trivial.
+    repeat (apply exist_ne => ?).
+    repeat apply sep_ne; trivial.
+    apply later_contractive => i H. by apply HP.
+  Qed.
+
+  Definition StackLink Q {HQ} := fixpoint (@StackLink_pre Q HQ).
+
+  Lemma StackLink_unfold Q {HQ} v :
+    @StackLink Q HQ v ≡
+              (∃ l w, v.1 = LocV l ★ l ↦ˢᵗᵏ w ★
+                                    ((w = InjLV UnitV ∧ v.2 = InjLV UnitV) ∨
+                                     (∃ y1 z1 y2 z2,
+                                         (w = InjRV (PairV y1 z1))
+                                           ★ (v.2 = InjRV (PairV y2 z2))
+                                           ★ Q (y1, y2)
+                                           ★ ▷ @StackLink Q HQ (z1, z2)
+                                     )
+                                    )
+              )%I.
+  Proof.
+    unfold StackLink at 1.
+    rewrite fixpoint_unfold; trivial.
+  Qed.
+
+  Global Opaque StackLink. (* So that we can only use the unfold above. *)
+
+  Lemma StackLink_dup_lem Q {HQ}:
+    True%I ⊢ (∀ v, @StackLink Q HQ v -★ @StackLink Q HQ v ★ @StackLink Q HQ v)%I.
+  Proof.
+    etrans; [|apply löb].
+    iIntros "Hlat".
+    rewrite later_forall.
+    iIntros {v} "H".
+    rewrite StackLink_unfold.
+    iDestruct "H" as {l w} "[% [Hl Hr]]"; subst.
+    iPoseProof (stack_mapsto_dup with "[Hl]") as "Hl'"; eauto.
+    iDestruct "Hl'" as "[Hl1 Hl2]".
+    iDestruct "Hr" as "[#Hr|Hr]".
+    {
+      iSplitL "Hl1".
+      - iExists _, _; iFrame "Hl1"; iSplitL; trivial; iLeft; trivial.
+      - iExists _, _; iFrame "Hl2"; iSplitL; trivial; iLeft; trivial.
+    }
+    {
+      iDestruct "Hr" as {y1 z1 y2 z2} "[#H1 [#H2 [#HQ H']]]".
+      iPoseProof ("Hlat" $! (z1, z2)) as "Hlat".
+      rewrite later_wand.
+      iPoseProof ("Hlat" with "H'") as "Hlat".
+      rewrite later_sep. iDestruct "Hlat" as "[HS1 HS2]".
+      iSplitL "Hl1 HS1".
+      - iExists _, _; iFrame "Hl1"; iSplitR; trivial.
+        iRight. iExists _, _, _, _; repeat iSplitR; trivial.
+      - iExists _, _; iFrame "Hl2"; iSplitR; trivial.
+        iRight. iExists _, _, _, _; repeat iSplitR; trivial.
+    }
+  Qed.
+
+  Lemma StackLink_dup Q {HQ} v :
+    @StackLink Q HQ v ⊢ (@StackLink Q HQ v ★ @StackLink Q HQ v)%I.
+  Proof. iIntros "H"; by iApply StackLink_dup_lem. Qed.
+
+  Lemma stackR_valid (h : stackR) (i : loc) :
+    ✓ h → h !! i = None ∨ ∃ v, h !! i = Some (DecAgree v).
+  Proof.
+    intros H; specialize (H i).
+    match type of H with
+      ✓ ?A => match goal with
+             | |- ?B = _ ∨ (∃ _, ?C = _) =>
+               change B with A; change C with A;
+                 destruct A as [[c|]|]; inversion H; eauto
+             end
+    end.
+  Qed.
+
+  Lemma stackR_alloc (h : stackR) (i : loc) (v : val) :
+    h !! i = None → (● h) ~~> (● (<[i := DecAgree v]> h)
+                               ⋅ ◯ {[i := DecAgree v]}).
+  Proof.
+    intros H1 n z H2. rewrite (insert_singleton_op h); auto.
+    destruct z as [[ze | |] zo];
+      unfold validN, cmra_validN in *; simpl in *; trivial.
+    destruct H2 as [H21 H22]; split.
+    - destruct H21 as [u H21].
+      eexists ({[i := DecAgree v]} ⋅ u). rewrite H21.
+      rewrite ?cmra_unit_left_id.
+      rewrite ?assoc.
+      rewrite (comm _ _ zo). apply cmra_op_ne'; trivial.
+      rewrite -assoc. by rewrite -stackR_self_op.
+    - intros j. rewrite lookup_op.
+      destruct (decide (i = j)) as [|Hneq]; subst.
+      + rewrite H1. rewrite lookup_singleton. constructor.
+      + rewrite lookup_singleton_ne; trivial.
+        specialize (H22 j).
+        revert H22.
+        match goal with
+          |- ✓{_} ?B → ✓{_} (_ ⋅ ?A) =>
+          change B with A; destruct A; by try constructor
+        end.
+  Qed.
+
+  Lemma option_dec_agree_equiv_eq (x y : option (dec_agreeR val)) :
+    x ≡ y → x = y.
+  Proof.
+    intros H1.
+    destruct x as [[x|]|]; destruct y as [[y|]|]; cbv in H1;
+      inversion H1; subst; auto with f_equal.
   Qed.
 
   Lemma dec_agree_valid_op_eq (x y : dec_agreeR val) :
@@ -49,7 +192,7 @@ Section Rules.
   Qed.
 
   Lemma stackR_auth_is_subheap (h h' : stackR) :
-    ✓ (● h ⋅ ◯ h') → ∀ i x, h' !! i ≡ Some x → h !! i ≡ Some x.
+    ✓ (● h ⋅ ◯ h') → ∀ i x, h' !! i = Some x → h !! i = Some x.
   Proof.
     intros H1 i x H2.
     destruct H1 as [H11 H12]; simpl in H11.
@@ -60,6 +203,7 @@ Section Rules.
     destruct H11 as [[z1 z2] [H31 [H32 H33]]]; simpl in *.
     specialize (H32 i).
     assert (H4 : ✓ (z1 ⋅ z2))by (by rewrite -H31).
+    apply option_dec_agree_equiv_eq.
     rewrite H31. rewrite lookup_op.
     specialize (H4 i). rewrite ?lookup_op in H4.
     revert H32; rewrite H2 => H32.
@@ -83,28 +227,97 @@ Section Rules.
     - inversion H1; subst. constructor; trivial.
   Qed.
 
-  Lemma stackR_alloc (h : stackR) (i : loc) (v : val) :
-    h !! i = None → (● h) ~~> (● ({[i := DecAgree v]} ⋅ h)).
+  Context {iI : heapIG Σ}.
+
+  Definition stack_owns (h : stackR) :=
+    (
+      (ghost_ownership.own stack_name (● h))
+        ★ Π★{map h} (λ l v, match v with
+                            | DecAgree v' => l ↦ᵢ v'
+                            | _ => True
+                            end)
+    )%I.
+
+  Lemma stack_owns_alloc E h l v :
+    ((stack_owns h ★ l ↦ᵢ v)%I)
+      ⊢ |={E}=> (stack_owns (<[l := DecAgree v]> h) ★ l ↦ˢᵗᵏ v)%I.
   Proof.
-    intros H1 n z H2.
-    destruct z as [[ze | |] zo];
-      unfold validN, cmra_validN in *; simpl in *; trivial.
-    destruct H2 as [H21 H22]; split.
-    - destruct H21 as [u H21].
-      eexists ({[i := DecAgree v]} ⋅ u). rewrite H21.
-      rewrite ?cmra_unit_left_id.
-      rewrite ?assoc.
-      by rewrite (comm _ zo).
-    - intros j. rewrite lookup_op.
-      destruct (decide (i = j)) as [|Hneq]; subst.
-      + rewrite H1. rewrite lookup_singleton; constructor.
-      + rewrite lookup_singleton_ne; trivial.
-        specialize (H22 j).
-        revert H22.
-        match goal with
-          |- ✓{_} ?B → ✓{_} (_ ⋅ ?A) =>
-          change B with A; destruct A; by try constructor
-        end.
+    iIntros "[[Hown Hall] Hl]".
+    iDestruct (own_valid _ with "Hown !") as "Hvalid".
+    iDestruct (auth_validI _ with "Hvalid") as "[Ha' Hb]";
+      simpl; iClear "Hvalid".
+    iDestruct "Hb" as %H1.
+    iDestruct "Ha'" as {h'} "Ha'"; iDestruct "Ha'" as %Ha'.
+    rewrite ->(left_id _ _) in Ha'; setoid_subst.
+    specialize (H1 l).
+    match type of H1 with
+      ✓ ?A => change A with (h' !! l) in H1
+    end.
+    destruct (h' !! l) as [[w|]|] eqn:Heq; inversion H1.
+    - rewrite <- (insert_delete _ _ _ Heq).
+      rewrite big_sepM_insert; [|apply lookup_delete_None; auto].
+      iDestruct "Hall" as "[Hl' Hall]".
+      iExFalso. iApply heap_mapsto_dup_invalid; by iFrame "Hl Hl'".
+    - iPvs (own_update with "Hown") as "Hown".
+      by apply stackR_alloc.
+      rewrite own_op. iDestruct "Hown" as "[Hown Hl']".
+      iPvsIntro. iSplitR "Hl'"; [|unfold stack_mapsto, auth_own; trivial].
+      iCombine "Hl" "Hall" as "Hall".
+      unfold stack_owns. iFrame "Hown".
+      rewrite big_sepM_insert; trivial.
+  Qed.
+
+  Lemma stack_owns_open h l v :
+    ((stack_owns h ★ l ↦ˢᵗᵏ v)%I)
+      ⊢ ((ghost_ownership.own stack_name (● h))
+           ★ Π★{map delete l h}
+           (λ l v,
+            match v with
+            | DecAgree v' => l ↦ᵢ v'
+            | DecAgreeBot => True
+            end)
+           ★ l ↦ᵢ v ★ l ↦ˢᵗᵏ v)%I.
+  Proof.
+    iIntros "[[Hown Hall] Hl]".
+    unfold stack_mapsto, auth_own.
+    iCombine "Hown" "Hl" as "Hown".
+    iDestruct (own_valid _ with "Hown !") as "Hvalid".
+    iDestruct "Hvalid" as %Hvalid.
+    rewrite own_op. iDestruct "Hown" as "[Hown Hl]".
+    assert (Heq : h !! l = Some (DecAgree v)).
+    eapply stackR_auth_is_subheap; eauto using lookup_singleton.
+    rewrite <- (insert_delete _ _ _ Heq).
+    rewrite big_sepM_insert; [|apply lookup_delete_None; auto].
+    iDestruct "Hall" as "[Hl' Hall]".
+    iFrame "Hl' Hown Hl". rewrite delete_insert; auto using lookup_delete.
+  Qed.
+
+  Lemma stack_owns_close h l v :
+    ((ghost_ownership.own stack_name (● h))
+       ★ Π★{map delete l h}
+       (λ l v,
+        match v with
+        | DecAgree v' => l ↦ᵢ v'
+        | DecAgreeBot => True
+        end)
+       ★ l ↦ᵢ v ★ l ↦ˢᵗᵏ v)%I ⊢ ((stack_owns h ★ l ↦ˢᵗᵏ v)%I).
+  Proof.
+    iIntros "[Hown [Hall [Hl Hl']]]".
+    unfold stack_mapsto, auth_own.
+    iCombine "Hown" "Hl'" as "Hown".
+    iDestruct (own_valid _ with "Hown !") as "Hvalid".
+    iDestruct "Hvalid" as %Hvalid.
+    rewrite own_op. iDestruct "Hown" as "[Hown Hl']".
+    assert (Heq : h !! l = Some (DecAgree v)).
+    eapply stackR_auth_is_subheap; eauto using lookup_singleton.
+    iCombine "Hl" "Hall" as "Hall".
+    rewrite -(big_sepM_insert (λ l v,
+        match v with
+        | DecAgree v' => (l ↦ᵢ v')%I
+        | DecAgreeBot => True%I
+        end) _ _ (DecAgree v)); eauto using lookup_delete.
+    rewrite insert_delete; auto using lookup_delete.
+    unfold stack_owns. by iFrame "Hown Hl' Hall".
   Qed.
 
 End Rules.
